ConcreteProg

Values.v
@@ -2,14 +2,22 @@ Definition ptr : Type := nat.
 
 Definition memdata : Type := nat.
 
-Inductive data_t : Set :=
-  | TInt
-  | TPtr.
-
-Definition data_ty (t : data_t) : Type :=
-  match t with
-  | TInt => nat
-  | TPtr => ptr
-  end.
-
 Definition mem : Type := ptr -> memdata.
+
+Module Mem.
+  Definition t := mem.
+
+  Definition read (m : t) (p : ptr) : memdata := m p.
+
+  (* TODO? Stdlib *)
+  Fixpoint ptr_eq (p0 p1 : ptr) {struct p0} : {p0 = p1}+{p0<>p1}.
+  Proof.
+    case p0 as [|p0], p1 as [|p1].
+    2,3:right; discriminate 1.
+    - left; reflexivity.
+    - case (ptr_eq p0 p1); [left|right]; congruence.
+  Defined.
+
+  Definition write (m : t) (p : ptr) (x : memdata) : t :=
+    fun p' => if ptr_eq p' p then x else m p'.
+End Mem.
