ConcreteProg.v
@@ -1,0 +1,213 @@
+Require Import Coq.Program.Equality.
+Require Import Coq.Relations.Relations.
+
+Require Export SLFun.Values.
+
+Definition fid : Set := nat.
+
+Inductive instr : Type -> Type :=
+  | Ret  [A] (x : A) : instr A
+  | Bind [A B] (f : instr A) (g : A -> instr B) : instr B
+  | Call [A] (R : Type) (f : fid) (x : A) : instr R
+  | Oracle (A : Type) : instr A
+  | Assert (P : mem -> Prop) : instr unit
+  (* Memory *)
+  | Read (p : ptr) : instr memdata
+  | Write (p : ptr) (x : memdata) : instr unit.
+
+Record f_impl := mk_f_impl {
+  f_arg_t : Type;
+  f_ret_t : Type;
+  f_body  : f_arg_t -> instr f_ret_t;
+}.
+
+Definition context := fid -> option f_impl.
+
+(* Small step semantics *)
+
+Section Semantics.
+
+  Variable G : context.
+
+  Definition state A := (mem * instr A)%type.
+
+  Inductive step : forall [A], state A -> state A -> Prop :=
+    | step_bind_l m m' [A B] (f f' : instr A) (g : A -> instr B)
+        (STEP_l : step (m, f) (m', f')):
+        step (m, Bind f g) (m', Bind f' g)
+    | step_bind_r m [A B] (x : A) (g : A -> instr B):
+        step (m, Bind (Ret x) g) (m, g x)
+    | step_call m f arg_t ret_t body x
+        (GET_F : G f = Some (mk_f_impl arg_t ret_t body)):
+        step (m, Call ret_t f x) (m, body x)
+    | step_assert m (P : mem -> Prop)
+        (ASSERT : P m):
+        step (m, Assert P) (m, Ret tt)
+    | step_read m p:
+        step (m, Read p) (m, Ret (Mem.read m p))
+    | step_write m p x:
+        step (m, Write p x) (Mem.write m p x, Ret tt).
+
+  Definition steps [A] : state A -> state A -> Prop :=
+    clos_refl_trans_n1 _ (@step A).
+
+  Definition okstate [A] (s : state A) :=
+    (exists x, snd s = Ret x) \/ (exists s', step s s').
+
+End Semantics.
+
+(* Specification and proof *)
+
+Fixpoint oracle_free [A] (i : instr A) : Prop :=
+  match i with
+  | Oracle _ => False
+  | Bind f g => oracle_free f /\ forall x, oracle_free (g x)
+  | _        => True
+  end.
+
+Definition context_oracle_free (c : context) :=
+  forall f fi, c f = Some fi -> forall x, oracle_free (f_body fi x).
+
+Record f_spec := mk_f_spec {
+  fs_arg_t : Type;
+  fs_ret_t : Type;
+  fs_pre   : fs_arg_t -> mem -> Prop;
+  fs_post  : fs_arg_t -> mem -> fs_ret_t -> mem -> Prop;
+}.
+
+Definition scontext := fid -> f_spec -> Prop.
+
+Section WLP.
+  Variable G : scontext.
+
+  Fixpoint wlp [A] (i : instr A) {struct i} : forall (post : A -> mem -> Prop) (m : mem), Prop :=
+    match i with
+    | Ret x => fun post =>
+        post x
+    | Bind f g => fun post =>
+        wlp f (fun y => wlp (g y) post)
+    | @Call A R f x => fun post m =>
+        exists fpre fpost, G f (mk_f_spec A R fpre fpost) /\
+        fpre x m /\
+        forall r m', fpost x m r m' -> post r m'
+    | Oracle A => fun post m =>
+        exists x : A, post x m
+    | Assert P => fun post m =>
+        P m /\ post tt m
+    | Read p => fun post m =>
+        post (Mem.read m p) m
+    | Write p x => fun post m =>
+        post tt (Mem.write m p x)
+    end.
+
+  Lemma wlp_monotone [A] (i : instr A) (post0 post1 : A -> mem -> Prop) m
+    (LE : forall x m, post0 x m -> post1 x m):
+    wlp i post0 m -> wlp i post1 m.
+  Proof.
+    revert post0 post1 m LE; induction i using instr_ind; do 4 intro; simpl;
+    try solve [apply LE | intuition eauto].
+    - (* Bind *)
+      apply IHi.
+      do 2 intro; apply H, LE.
+    - (* Call *)
+      intros (? & ? & ? & ? & IMP).
+      do 2 eexists; do 2 (esplit; [eassumption|]).
+      intros; apply LE, IMP; assumption.
+    - (* Oracle *)
+      intros (? & P); eauto.
+  Qed.
+
+  Inductive f_match_spec : f_impl -> f_spec -> Prop :=
+    | intro_match_spec arg_t res_t (pre : arg_t -> mem -> Prop) post body
+        (MATCH : forall x m, pre x m -> wlp (body x) (post x m) m):
+        f_match_spec (mk_f_impl arg_t res_t body) (mk_f_spec arg_t res_t pre post).
+End WLP.
+
+Section WLP_Correct.
+  Variables (C : context) (S : scontext).
+
+  Definition context_match_spec : Prop :=
+    forall f fs, S f fs -> exists fi, C f = Some fi /\ f_match_spec S fi fs.
+
+  Hypothesis MATCH : context_match_spec.
+
+  Lemma match_init_call f ret_t arg_t pre post body x m
+    (FI : C f = Some (mk_f_impl arg_t ret_t body))
+    (FS : S f (mk_f_spec arg_t ret_t pre post))
+    (PRE : pre x m):
+    wlp S (body x) (post x m) m.
+  Proof.
+    apply MATCH in FS as (fi' & FI' & SF).
+    rewrite FI in FI'; injection FI' as ?; subst fi'.
+    dependent destruction SF.
+    apply MATCH0, PRE.
+  Qed.
+
+  Lemma wlp_preserved A s s' (post : A -> mem -> Prop):
+    step C s s' ->
+    wlp S (snd s) post (fst s) -> wlp S (snd s') post (fst s').
+  Proof.
+    induction 1; simpl; try solve [intuition auto].
+    - (* Call *)
+      intros (fpre & fpost & SF & PRE & POST).
+      eapply match_init_call in PRE; try eassumption.
+      eapply wlp_monotone; eassumption.
+  Qed.
+
+  Lemma wlp_step A m i (post : A -> mem -> Prop)
+    (WLP : wlp S i post m)
+    (OFREE : oracle_free i):
+    okstate C (m, i).
+  Proof.
+    unfold okstate; induction i; simpl in *.
+    1:left; eauto. (* Ret *)
+    all:right; try solve [case OFREE | intuition eauto using step].
+    - (* Bind *)
+      ecase IHi as [(? & ->)|((?,?) & STEP)]. apply WLP. apply OFREE.
+      all:eauto using step.
+    - (* Call *)
+      case WLP as (fpre & fpost & SP & _ & _).
+      apply MATCH in SP as (fi & IM & MT); inversion MT; subst.
+      eauto using step.
+  Qed.
+
+  Hypothesis COFREE : context_oracle_free C.
+
+  Lemma ofree_preserved A s s'
+    (OFREE : @oracle_free A (snd s)):
+    step C s s' -> oracle_free (snd s').
+  Proof.
+    induction 1; simpl in *; intuition auto.
+    - (* Call *)
+      apply COFREE in GET_F.
+      apply GET_F.
+  Qed.
+
+  Lemma wlp_stars_okstate A s s' post
+    (OFREE : @oracle_free A (snd s))
+    (WLP : wlp S (snd s) post (fst s))
+    (STEPS : steps C s s'):
+    okstate C s'.
+  Proof.
+    assert (H : wlp S (snd s') post (fst s') /\ oracle_free (snd s')). {
+      induction STEPS; auto.
+      destruct IHSTEPS.
+      eauto using wlp_preserved, ofree_preserved.
+    }
+    case s' as (m, i).
+    eapply wlp_step; apply H. 
+  Qed.
+
+  Lemma func_okstate f arg_t ret_t pre post body x m s'
+    (FI : C f = Some (mk_f_impl arg_t ret_t body))
+    (FS : S f (mk_f_spec arg_t ret_t pre post))
+    (PRE : pre x m)
+    (STEPS : steps C (m, body x) s'):
+    okstate C s'.
+  Proof.
+    eapply match_init_call in PRE; try eassumption.
+    eapply wlp_stars_okstate, STEPS.
+    - eapply COFREE in FI. apply FI.
+    - exact PRE.
+  Qed.
+End WLP_Correct.
