Test/Concrete.v
@@ -1,0 +1,83 @@
+Require Import SLFun.ConcreteProg.
+
+Definition f_aux  : fid := 0.
+Definition f_main : fid := 1.
+
+Definition s_aux : f_spec := {|
+  fs_arg_t := ptr;
+  fs_ret_t := nat;
+  fs_pre   := fun p m => Mem.read m p > 0;
+  fs_post  := fun p m0 r m1 => Mem.read m1 p = S r;
+|}.
+
+Definition s_main : f_spec := {|
+  fs_arg_t := unit;
+  fs_ret_t := unit;
+  fs_pre   := fun _ _ => True;
+  fs_post  := fun _ _ _ _ => True;
+|}.
+
+Inductive Sctx : scontext :=
+  | Sctx_aux  : Sctx f_aux  s_aux
+  | Sctx_main : Sctx f_main s_main.
+
+Definition i_aux : f_impl := {|
+  f_arg_t := ptr;
+  f_ret_t := nat;
+  f_body  := fun p =>
+    Bind (Read p) (fun x => Ret (pred x))
+|}.
+
+Definition ptr0 : ptr := 42.
+Global Opaque ptr0.
+
+Definition i_main : f_impl := {|
+  f_arg_t := unit;
+  f_ret_t := unit;
+  f_body  := fun _ =>
+    Bind (Write ptr0 3) (fun _ =>
+    Bind (Call nat f_aux ptr0) (fun r =>
+          Assert (fun m => Mem.read m ptr0 = S r)))
+|}.
+
+Definition Cctx : context :=
+  fun f => match f with
+  | 0 => Some i_aux
+  | 1 => Some i_main
+  | _ => None
+  end.
+
+Lemma match_aux:
+  f_match_spec Sctx i_aux s_aux.
+Proof.
+  constructor; intros p m; simpl.
+  case (Mem.read m p); simpl; try reflexivity.
+  inversion 1.
+Qed.
+
+Lemma match_main:
+  f_match_spec Sctx i_main s_main.
+Proof.
+  constructor; intros _ m _; simpl.
+  do 3 esplit. constructor.
+  simpl.
+  split.
+    { unfold Mem.read, Mem.write; destruct Mem.ptr_eq.
+      repeat constructor. congruence. }
+  auto.
+Qed.
+
+Lemma match_context:
+  context_match_spec Cctx Sctx.
+Proof.
+  inversion 1; simpl; (do 2 esplit; [reflexivity|]).
+  apply match_aux.
+  apply match_main.
+Qed.
+
+Lemma context_oracle_free:
+  context_oracle_free Cctx.
+Proof.
+  intros [|[|]] fi; simpl; simplify_eq 1; intros <- ?;
+  repeat constructor.
+Qed.
