Util.v
@@ -1,0 +1,12 @@
+Ltac symmetric_iff :=
+  let H  := fresh "H"  in
+  eassert _ as H; [|
+    let Hs := fresh "Hs" in
+    pose proof (Hs := H);
+    repeat (let x := fresh "x" in intro x;
+            refine (_ (Hs x)); clear Hs; intro Hs);
+    split; [ exact Hs
+           | eapply H; try solve [try symmetry; eassumption] ];
+    clear H Hs
+  ].
+
